\documentclass[a4paper, 12 pt]{article}

\usepackage[english, russian]{babel}
\usepackage[T2A]{fontenc}
\usepackage[utf8]{inputenc}
\usepackage{geometry}

\geometry{top=4ex}
\geometry{bottom=4ex}
\geometry{left=5em}
\geometry{right=5em}

\author{Муратов Артём}
\date{3Б класс}
\title{Домашняя работа}
\maketitle

№9(1) Вычислить:	\[\left((\left(2\right)^{(\left(2\right){\cdot}x)})\right)'
\]


Решение:

Очевидно,
	\[\left(x\right)'
	= \left(1\right)\]
Пока примем без доказательства, что:
	\[\left(\left(2\right)\right)'
	= \left(0\right)\]
Заметим, что:
	\[\left((\left(2\right){\cdot}x)\right)'
	= ((\left(0\right){\cdot}x)+(\left(2\right){\cdot}\left(1\right)))\]
Пока примем без доказательства, что:
	\[\left(ln{\left(2\right)}\right)'
	= \left(0\right)\]
Заметим, что:
	\[\left((ln{\left(2\right)}{\cdot}(\left(2\right){\cdot}x))\right)'
	= ((\left(0\right){\cdot}(\left(2\right){\cdot}x))+(ln{\left(2\right)}{\cdot}((\left(0\right){\cdot}x)+(\left(2\right){\cdot}\left(1\right)))))\]
После простых преобразований:
	\[\left((\left(2\right)^{(\left(2\right){\cdot}x)})\right)'
	= ((\left(2\right)^{(\left(2\right){\cdot}x)}){\cdot}((\left(0\right){\cdot}(\left(2\right){\cdot}x))+(ln{\left(2\right)}{\cdot}((\left(0\right){\cdot}x)+(\left(2\right){\cdot}\left(1\right))))))\]
Упростив выражение получаем ответ:
	\[\left((\left(2\right)^{(\left(2\right){\cdot}x)})\right)'
	= ((\left(2\right)^{(\left(2\right){\cdot}x)}){\cdot}\left(1.38629\right))\]

\end{document}
